Up-to bind for CTrees (WIP)

CTree.v
@@ -9,7 +9,7 @@ From RelationAlgebra Require Import
      normalisation
      monoid.
 From CTree Require Import CTree Eq Eq.Epsilon.
-From OptSim Require Import Utils LTS OptSim.
+From OptSim Require Import (*Trace*) Utils LTS Divergence OptSim.
 
 Import CoindNotations.
 
@@ -28,87 +28,315 @@ Definition clabel {E} (l : @LTS.label (@olabel E)) :=
 Program Definition lts {E B X} : LTS :=
 {|
   Observable := @olabel E;
-  St := @SS E B X;
+  St := @SS E B X; (* FIXME heterogeneous ctrees *)
   LTS.trans := fun l => {| hrel_of := Trans.trans (clabel l) |};
   (*epsilon := {| hrel_of := fun _ _ => False |};*)
   Robs := eq; (* FIXME heterogeneous relations *)
   ub_state := fun _ => False
 |}.
 
-#[export] Instance Chain_simF_equ E B X freeze lock delay b : forall (R : Chain (simF (lts := lts) freeze lock delay)),
+#[export] Instance Chain_simF_equ {E B X} freeze lock delay b : forall (R : Chain (simF (lts := lts) freeze lock delay)),
   Proper (@equ E B X X eq ==> equ eq ==> impl) (`R b).
 Proof.
   intros. cbn. intros.
   eapply (Chain_simF_eq'' (lts := lts)); eauto.
 Qed.
 
-Lemma ObsAnswer_bind_r : forall E B X Y delay R (s' : St (@lts E B Y)) (t : St (@lts E B X)) (k : X -> ctree E B Y) x o,
+Lemma dtrans_bind_l : forall {E B X Y} delay l (t t' : St (@lts E B X)) (k : X -> ctree E B Y)
+  (LBL : ~is_val (clabel l)),
+  dtrans (lts := lts) delay l t t' ->
+  dtrans (lts := @lts E B Y) delay l (CTree.bind t k) (CTree.bind t' k).
+Proof.
+  intros. apply dtrans_case in H as [| [-> ?]].
+  - apply trans_dtrans. apply trans_bind_l; auto.
+  - destruct H. rewrite str_itr' in H. esplit.
+    apply transs_bind_l. apply H.
+    apply trans_bind_l; auto.
+Qed.
+
+(* WRONG because Br: k x is not necessarily visible *)
+Lemma taustar_bind_r : forall {E B X Y} (u : St (@lts E B Y)) (t : St (@lts E B X)) (k : X -> ctree E B Y) x,
+  (((trans tau)^*)⋅trans (lts := lts) (LTS.obs (oval x))) t Stuck ->
+  (trans (lts := lts) tau)^* (k x) u ->
+  (trans (lts := lts) tau)^* (CTree.bind t k) u.
+Proof.
+  (*intros. assert (wtrans τ (CTree.bind t k) u).
+  2: { now apply wtrans_τ. }
+  destruct H. eapply wtrans_bind_r'. eapply wconss. apply wtrans_τ. apply H. apply trans_wtrans. apply H1. Search pwtrans. eapply transs_bind
+  intros. revert H0. eapply srel_str_ind_r with (i := trans tau) (P := fun u => (trans (lts := lts) tau)^* (k x) u -> (trans (lts := lts) tau)^* (CTree.bind t k) u).
+  3: { rewrite <- str_refl. reflexivity. }
+  3: {*)
+Abort.
+
+Lemma dtrans_bind_r : forall {E B X Y} delay l (u : St (@lts E B Y)) (t : St (@lts E B X)) (k : X -> ctree E B Y) x,
+  dtrans (lts := lts) delay (LTS.obs (oval x)) t Stuck ->
+  dtrans (lts := lts) delay l (k x) u ->
+  dtrans delay l (CTree.bind t k) u.
+Proof.
+  intros. destruct delay.
+  - cbn -[dot str trans].
+    red in H, H0.
+    intros. destruct H, H0.
+    rewrite str_itr in H0.
+    destruct H0.
+    + esplit. apply transs_bind_l with (k := k) in H. apply H.
+      eapply trans_bind_r. apply H1. cbn in H0. rewrite H0. apply H2.
+    + esplit. 2: apply H2. rewrite <- str_trans. esplit.
+      * apply transs_bind_l with (k := k) in H. apply H.
+      * rewrite itr_str_l in H0.
+        rewrite <- str_itr'.
+        rewrite itr_str_l. destruct H0. esplit. 2: apply H3.
+        eapply trans_bind_r. apply H1. apply H0.
+  - cbn. eapply trans_bind_r. apply H. apply H0.
+Qed.
+
+Lemma tauplus_bind_l : forall {E B X Y} (t t' : St (@lts E B X)) (k : X -> ctree E B Y),
+  (lts.(trans) tau)^+ t t' ->
+  (lts.(trans) tau)^+ (CTree.bind t k) (CTree.bind t' k).
+Proof.
+  intros. apply dtrans_tauplus with (delay := SimOpt.delay).
+  apply tauplus_dtrans in H.
+  eapply dtrans_bind_l; eauto. apply is_val_τ.
+Qed.
+
+Lemma tauplus_bind_r : forall {E B X Y} (u : St (@lts E B Y)) (t : St (@lts E B X)) (k : X -> ctree E B Y) x,
+  dtrans (lts := lts) SimOpt.delay(*FIXME*) (LTS.obs (oval x)) t Stuck ->
+  (lts.(trans) tau)^+ (k x) u ->
+  (lts.(trans) tau)^+ (CTree.bind t k) u.
+Proof.
+  intros. apply dtrans_tauplus with (delay := SimOpt.delay).
+  apply tauplus_dtrans in H0.
+  eapply dtrans_bind_r; eauto.
+Qed.
+
+Lemma ObsAnswer_bind_r : forall {E B X Y} delay R (s' : St (@lts E B Y)) (t : St (@lts E B X)) (k : X -> ctree E B Y) x o,
   ObsAnswer (lts := lts) delay (fun _ _ => True) Stuck t (oval x) ->
   ObsAnswer delay R s' (k x) o ->
   ObsAnswer delay R s' (CTree.bind t k) o.
 Proof.
   intros. destruct H.
-  - cbn in OBS. subst.
-    destruct H0.
-    + eapply ans_obs; try eassumption. eapply trans_bind_r.
-      apply trans_val_inv in TR as ?. rewrite H in TR. apply TR.
-      apply TR0.
-Admitted.
+  cbn in OBS. subst.
+  destruct H0. eapply ans_obs. eapply dtrans_bind_r; eauto.
+  all: auto.
+  apply dtrans_trans in TR as ?. destruct H.
+  apply trans_val_inv in H0.
+  now rewrite H0 in TR.
+Qed.
 
-Lemma epsilon_correct : forall E B X (t u : ctree E B X),
+Lemma epsilon_correct : forall {E B X} (t u : ctree E B X),
   Epsilon.epsilon t u ->
-  OptSim.epsilon (lts := lts) t u.
+  LTS.epsilon (lts := lts) t u.
 Proof.
   red. intros.
   eapply epsilon_trans; eauto.
 Qed.
 
-Lemma TauAnswer_bind_r : forall E B X Y freeze lock delay (R : Chain (simF freeze lock delay))
-  (s' : St (@lts E B Y)) (t : St (@lts E B X)) (k : X -> ctree E B Y) x,
+Lemma TauAnswer_bind_r : forall {E B X Y} freeze lock delay (R : Chain (simF freeze lock delay))
+  (s' : St (@lts E B Y)) (t : St (@lts E B X)) (k : X -> ctree E B Y) x
+  (Hlock : lock = SimOpt.nolock \/ forall x, extrans (lts := lts) (k x)),
   ObsAnswer (lts := lts) delay (fun _ _ => True) Stuck t (oval x) ->
   TauAnswer freeze delay (`R true) (`R false) s' (k x) ->
   TauAnswer freeze delay (`R true) (`R false) s' (CTree.bind t k).
 Proof.
   intros. destruct H.
-  - cbn in OBS. subst.
-    destruct H0.
+  cbn in OBS. subst. assert (t' ≅ Stuck). {
+    apply dtrans_trans in TR as [].
+    now apply trans_val_inv in H1.
+  }
+  rewrite H in TR. clear t' H.
+  apply dtrans_case in TR as [TR | [-> TR]].
+  - destruct H0.
     + eapply tau_exact; try eassumption. eapply trans_bind_r.
-      apply trans_val_inv in TR as ?. rewrite H in TR. apply TR.
-      apply TR0.
+      apply TR. apply TR0.
     + apply tau_freeze; auto.
-      eapply upto_epsilon_r. admit. 2: apply SIM0.
+      eapply upto_epsilon_r. auto. 3: apply SIM0.
+      { destruct Hlock; auto. }
       apply epsilon_correct. eapply epsilon_bind_ret.
       now apply trans_val_epsilon in TR as [].
     + apply tau_div'; auto. intro.
-      eapply upto_epsilon_r. admit. 2: destruct b; eauto.
+      eapply upto_epsilon_r. auto. 3: destruct b; eauto.
+      { destruct Hlock; auto. }
       apply epsilon_correct. eapply epsilon_bind_ret.
       now apply trans_val_epsilon in TR as [].
-    + eapply tau_delay; try eassumption. admit.
-  - admit.
-Admitted.
+    + eapply tau_delay; try eassumption.
+      eapply tauplus_bind_r; eauto.
+      apply trans_dtrans. apply TR.
+  - destruct H0.
+    + eapply tau_delay. auto.
+      eapply tauplus_bind_r.
+      * red. rewrite <- str_itr'. apply TR.
+      * rewrite <- itr_ext. apply TR0.
+      * apply SIM0.
+    + destruct TR.
+      eapply tau_delay. auto.
+      eapply tauplus_bind_l; eauto.
+      eapply upto_epsilon_r; eauto.
+      { destruct Hlock; auto. }
+      eapply epsilon_correct. eapply epsilon_bind_ret.
+      apply trans_val_epsilon in H1 as []. apply H1.
+    + destruct TR.
+      eapply tau_delay. auto.
+      eapply tauplus_bind_l; eauto.
+      eapply upto_epsilon_r; eauto.
+      { destruct Hlock; auto. }
+      eapply epsilon_correct. eapply epsilon_bind_ret.
+      apply trans_val_epsilon in H1 as []. apply H1.
+    + destruct TR.
+      eapply tau_delay. auto.
+      eapply tauplus_bind_r; eauto.
+      * esplit; eauto. rewrite <- str_itr'. apply H0.
+      * apply SIM0.
+Qed.
 
-Lemma upto_bind E B X Y freeze lock delay : forall
+Lemma diverges_bind {E B X Y} :
+  forall (t : ctree E B X) (k : X -> ctree E B Y),
+  diverges (lts := lts) t ->
+  diverges (lts := lts) (CTree.bind t k).
+Proof.
+  red. coinduction R CH. intros.
+  apply (gfp_fp divergesF) in H as (? & ? & ?).
+  exists (CTree.bind x k). split; auto. apply trans_bind_l; auto.
+  apply is_val_τ.
+Qed.
+
+Lemma divpres_upto_bind1 {E B X Y} freeze lock delay : forall
   (R : Chain (simF (lts := lts) freeze lock delay))
-  b (t t' : ctree E B X) (k k' : X -> ctree E B Y),
-  sim (lts := lts) freeze lock delay b t t' ->
-  (forall x, `R b (k x) (k' x)) ->
-  `R b (CTree.bind t k) (CTree.bind t' k').
+  (t : ctree E B X) (k k' : X -> ctree E B Y)
+  (Hlock : True(*lock = SimOpt.nolock \/ forall x, extrans (lts := lts) (k' x)*)),
+  True ->
+  (forall x, `R false (k x) (k' x)) ->
+  `R false (CTree.bind t k) (CTree.bind t k').
+Proof.
+  intro. apply tower. {
+    intros ??????????. apply H; auto.
+    intros. now apply H1.
+  }
+  clear R. intros R **.
+  apply simF_equiv.
+  constructor. intros ??. apply trans_bind_inv in H2 as [(? & ? & ? & ?)|(? & ? & ?)].
+  - subs.
+    eapply dtau_match. eapply trans_bind_l; eauto. apply H; auto. intros. step. apply H1.
+  - clear H0. assert (H0 : True) by apply I. specialize (H1 x). apply simF_equiv in H1.
+    revert s' H3.
+    assert (divpresF (`R false) (k x) (CTree.bind t k')).
+    2: { apply H3. }
+    remember (k x) as kx. assert (KX: (lts.(trans) tau)^* (k x) kx). { subst. now rewrite <- str_refl. } clear Heqkx.
+    remember (k' x) as k'x.
+    revert k k' x KX Hlock Heqk'x H2. induction H1; intros; subst.
+    constructor. intros ??.
+    apply H1 in H3 as ?. destruct H4.
+    + eapply dtau_plus. 2: { apply DIV. }
+      rewrite <- itr_ext. eapply trans_bind_r; eauto.
+    + destruct DIV.
+      eapply dtau_div. destruct DIV.
+      eapply H5; eauto.
+      rewrite str_unfold_r. right. esplit; eauto.
+Qed.
+
+Lemma divpres_upto_bind' {E B X Y} freeze lock : forall
+  (R : Chain (simF (lts := lts) freeze lock SimOpt.delay))
+  (t t' : ctree E B X) (k k' : X -> ctree E B Y),
+  (nodiv (lts := lts) t \/ diverges (lts := lts) t') ->
+  (forall x, `R false (k x) (k' x)) ->
+  (forall x : X, dtrans (lts := lts) SimOpt.delay (obs (oval x)) t Stuck -> dtrans (lts := lts) SimOpt.delay (obs (oval x)) t' Stuck) ->
+  `R false (CTree.bind t k) (CTree.bind t' k').
 Proof.
   intro. apply tower. {
     intros ???????????. apply H; auto.
     intros. now apply H1.
   }
-  clear R. intros R **. destruct b.
-  2: { admit. }
+  clear R. intros R **.
+  destruct H0.
+  2: { apply (gfp_bchain R). apply diverges_divpres. now apply diverges_bind. }
+  apply simF_equiv. induction H0.
+  constructor. intros ??.
+  apply trans_bind_inv in H4 as [(? & ? & ? & ?)|(? & ? & ?)].
+  - subs. apply H3 in H5 as ?. apply dtau_div. apply H6.
+    { intros. apply H2. red in H6 |- *. rewrite str_unfold_l, dotplsx. right.
+      rewrite <- dotA. esplit; eauto.
+    }
+  - specialize (H1 x). apply simF_equiv in H1. revert s' H5.
+    assert (divpresF (`R false) (k x) (CTree.bind t' k')).
+    2: { apply H5. }
+    remember (k x) as kx. assert (KX: (lts.(trans) tau)^* (k x) kx). { subst. now rewrite <- str_refl. } clear Heqkx.
+    remember (k' x) as k'x.
+    revert k k' x KX Heqk'x H3 H4. induction H1; intros; subst.
+    constructor. intros ??.
+    apply H1 in H5 as ?. destruct H6.
+    + eapply dtau_plus. 2: { apply DIV. }
+      specialize (H2 x). lapply H2.
+      2: { now apply trans_dtrans. }
+      clear H2. intro. eapply tauplus_bind_r; eauto.
+      rewrite <- itr_ext. apply TR.
+    + destruct DIV.
+      eapply dtau_div. destruct DIV.
+      eapply H7; eauto.
+      rewrite str_unfold_r. right. esplit; eauto.
+Qed.
+
+(* requires the excluded middle *)
+Lemma divpres_upto_bind {E B X Y} freeze lock : forall
+  (R : Chain (simF (lts := lts) freeze lock SimOpt.delay))
+  (t t' : ctree E B X) (k k' : X -> ctree E B Y),
+  (sim (lts := lts) SimOpt.freeze_div lock SimOpt.delay true t t') ->
+  (forall x, `R false (k x) (k' x)) ->
+  `R false (CTree.bind t k) (CTree.bind t' k').
+Proof.
+  intros. eapply divpres_upto_bind'; auto.
+  eapply divpres_case; eauto. apply sim_f_t; eauto.
+  intros. red in H1 |- *.
+  destruct H1. eapply sim_inv_taustar_l in H; eauto.
+  apply sim_fp in H. apply H in H2 as [].
+  cbn in OBS. subst.
+  red in TR. destruct TR. esplit; eauto.
+  apply trans_val_inv in H3 as ?. now subs.
+Qed.
+
+Lemma is_stuck_bind_inv {E B X Y} : forall (t : ctree E B X) (k : X -> ctree E B Y),
+  is_stuck (lts := lts) (CTree.bind t k) ->
+  is_stuck (lts := lts) t \/ forall l t', lts.(trans) l t t' -> exists r : X, l = obs (oval r) /\ t' ≅ Stuck.
+Proof.
+  intros.
+  destruct (Classical_Prop.classic (extrans (lts := lts) t)); auto.
+  right. intros.
+  destruct l.
+  2: {
+    apply trans_bind_l with (k := k) in H1. 2: apply is_val_τ.
+    exfalso. apply H. eexists; apply H1.
+  }
+  destruct s.
+  1: {
+    apply trans_bind_l with (k := k) in H1. 2: apply is_val_obs.
+    exfalso. apply H. eexists; apply H1.
+  }
+  apply trans_val_invT in H1 as ?. subst.
+  exists x. split; auto.
+  now apply trans_val_inv in H1.
+Qed.
+
+Lemma upto_bind E B X Y freeze lock delay (TMP : freeze <> SimOpt.freeze_div \/ delay = SimOpt.delay) : forall
+  (R : Chain (simF (lts := lts) freeze lock delay))
+  (t t' : ctree E B X) (k k' : X -> ctree E B Y)
+  (Hlock : lock = SimOpt.nolock \/ forall x, extrans (lts := lts) (k' x)),
+  (sim (lts := lts) freeze lock delay true t t') ->
+  (forall x, `R true (k x) (k' x)) ->
+  `R true (CTree.bind t k) (CTree.bind t' k').
+Proof.
+  intro. apply tower. {
+    intros ???????????. apply H; auto.
+    intros. now apply H1.
+  }
+  clear R. intros R **.
   apply simF_equiv. repeat split; intros.
   - (* observable transition *)
     apply trans_bind_inv in H2 as [(? & ? & ? & ?) | (? & ? & ?)].
     + (* transition from t *)
-      subs. apply sim_fp in H0. apply H0 in H3 as [].
-      * eapply ans_obs. eapply trans_bind_l in TR. apply TR. admit.
+      subs. apply sim_fp in H0. apply H0 in H3 as []. apply dtrans_case in TR as [TR | [-> TR]].
+      * eapply ans_obs. eapply trans_bind_l in TR. apply trans_dtrans. apply TR. cbn in OBS. subst. apply H2.
         apply itr_ext_hrel.
         apply H; auto. apply itr_sim; auto. typeclasses eauto. intros. step. apply H1. apply OBS.
-      * eapply ans_delay_obs; auto. instantiate (1 := (CTree.bind t'0 k')). admit.
+      * eapply ans_obs; auto. instantiate (1 := (CTree.bind t'0 k')).
+        { apply dtrans_bind_l; auto. cbn in OBS. subst. now rewrite str_itr' in TR. }
         apply itr_ext_hrel. apply H; auto. intros. apply itr_sim, SIM. typeclasses eauto.
         intros. step. apply H1.
     + (* transition from k *)
@@ -121,20 +349,41 @@ Proof.
     apply trans_bind_inv in H2 as [(? & ? & ? & ?) | (? & ? & ?)].
     + (* transition from t *)
       subs. apply sim_fp in H0. apply H0 in H3 as [].
-      * eapply tau_exact. eapply trans_bind_l in TR. apply TR. admit.
+      * eapply tau_exact. eapply trans_bind_l in TR. apply TR. apply is_val_τ.
         apply H; auto. intros. step. apply H1.
       * apply tau_freeze; auto.
         apply H; auto. intros. step. apply H1.
       * apply tau_div; auto. (* TODO simF_step_t *)
         apply H; auto. intros. step. apply H1.
-        apply H; auto. intros. apply simF_f_t. now subst. apply H1.
-      * eapply tau_delay; auto. instantiate (1 := (CTree.bind t'0 k')). admit.
+        subst. destruct TMP, delay; try easy.
+        eapply divpres_upto_bind; eauto.
+        intros. now apply simF_f_t.
+      * eapply tau_delay. auto. instantiate (1 := (CTree.bind t'0 k')).
+        { apply tauplus_bind_l; auto. }
         apply H; auto. intros. step. apply H1.
     + (* transition from k *)
       apply sim_fp in H0.
-      eapply TauAnswer_bind_r.
+      eapply TauAnswer_bind_r. auto.
       * lapply (proj1 H0 (oval x) Stuck). 2: { apply H2. }
         intros. eapply ObsAnswer_mon; eauto. cbn. auto.
       * specialize (H1 x). apply simF_equiv in H1. apply (proj1 (proj2 H1) s'). apply H3.
-  - admit.
+  - red. destruct Hlock; auto.
+    apply sim_fp in H0 as ?. destruct H3 as (_ & _ & []); auto.
+    right. intro. red.
+    apply is_stuck_bind_inv in H4 as [].
+    + apply H3 in H4. destruct delay.
+      * red in H4. destruct H4.
+        { left. Fail apply is_stuck_bind. admit. }
+        destruct H4 as (_ & ? & ? & ?).
+        right. split; auto.
+        eapply transs_bind_l with (k := k') in H4.
+        exists (CTree.bind x k'). split; auto.
+        Fail apply is_stuck_bind. admit.
+      * destruct H4; try easy.
+        left. Fail apply is_stuck_bind. admit.
+    + admit.
+    (* if t stuck then t' can be stuck so bind t' k' too OK.
+      if t pure, it means for all (k x) reachable (k x) is stuck,
+      so k' x can be stuck (one is enough) so bind t' k' is stuck.
+      I may need the excluded middle? *)
 Admitted.
